Added an is value flag to Stack

04Stack/Stack.thy
@@ -7,7 +7,7 @@ datatype frame =
   | FApp2 dexpr
   | FReturn
 
-datatype stack_state = SS "frame list" dexpr
+datatype stack_state = SS bool "frame list" dexpr
 
 inductive typecheck_stack :: "frame list \<Rightarrow> ty \<Rightarrow> ty \<Rightarrow> bool" (infix ": _ \<rightarrow>" 50) where
   tcs_nil [simp]: "[] : t \<rightarrow> t"
@@ -21,45 +21,55 @@ inductive_cases [elim]: "FApp2 e # s : t' \<rightarrow> t"
 inductive_cases [elim]: "FReturn # s : t' \<rightarrow> t"
 
 inductive typecheck_stack_state :: "stack_state \<Rightarrow> ty \<Rightarrow> bool" (infix ":\<^sub>s" 50) where
-  tcs_state [simp]: "s : t' \<rightarrow> t \<Longrightarrow> [] \<turnstile>\<^sub>d e : t' \<Longrightarrow> SS s e :\<^sub>s t"
+  tcs_state [simp]: "s : t' \<rightarrow> t \<Longrightarrow> [] \<turnstile>\<^sub>d e : t' \<Longrightarrow> (b \<Longrightarrow> vald e) \<Longrightarrow> SS b s e :\<^sub>s t"
 
-inductive_cases [elim]: "SS s e :\<^sub>s t"
+inductive_cases [elim]: "SS b s e :\<^sub>s t"
 
 inductive evals :: "stack_state \<Rightarrow> stack_state \<Rightarrow> bool" (infix "\<leadsto>\<^sub>s" 50) where
-  evs_app1 [simp]: "SS s (DApp e\<^sub>1 e\<^sub>2) \<leadsto>\<^sub>s SS (FApp1 e\<^sub>2 # s) e\<^sub>1"
-| evs_app2 [simp]: "vald e\<^sub>1 \<Longrightarrow> SS (FApp1 e\<^sub>2 # s) e\<^sub>1 \<leadsto>\<^sub>s SS (FApp2 e\<^sub>1 # s) e\<^sub>2"
-| evs_app3 [simp]: "vald e\<^sub>2 \<Longrightarrow> SS (FApp2 (DLam t e\<^sub>1) # s) e\<^sub>2 \<leadsto>\<^sub>s SS (FReturn # s) (substd 0 e\<^sub>2 e\<^sub>1)"
-| evs_ret [simp]: "vald e \<Longrightarrow> SS (FReturn # s) e \<leadsto>\<^sub>s SS s e"
+  evs_const [simp]: "SS False s (DConst k) \<leadsto>\<^sub>s SS True s (DConst k)"
+| evs_lam [simp]: "SS False s (DLam t e) \<leadsto>\<^sub>s SS True s (DLam t e)"
+| evs_app1 [simp]: "SS False s (DApp e\<^sub>1 e\<^sub>2) \<leadsto>\<^sub>s SS False (FApp1 e\<^sub>2 # s) e\<^sub>1"
+| evs_app2 [simp]: "SS True (FApp1 e\<^sub>2 # s) e\<^sub>1 \<leadsto>\<^sub>s SS False (FApp2 e\<^sub>1 # s) e\<^sub>2"
+| evs_app3 [simp]: "SS True (FApp2 (DLam t e\<^sub>1) # s) e\<^sub>2 \<leadsto>\<^sub>s SS False (FReturn # s) (substd 0 e\<^sub>2 e\<^sub>1)"
+| evs_ret [simp]: "SS True (FReturn # s) e \<leadsto>\<^sub>s SS True s e"
 
-lemma [simp]: "[] \<turnstile>\<^sub>d e : t \<Longrightarrow> \<not> vald e \<Longrightarrow> \<exists>\<Sigma>'. SS s e \<leadsto>\<^sub>s \<Sigma>'"
+lemma [simp]: "[] \<turnstile>\<^sub>d e : t \<Longrightarrow> \<exists>\<Sigma>'. SS False s e \<leadsto>\<^sub>s \<Sigma>'"
 proof (induction "[] :: ty list" e t rule: typecheckd.induct)
+  case (tcd_const k)
+  have "SS False s (DConst k) \<leadsto>\<^sub>s SS True s (DConst k)" by simp
+  thus ?case by fastforce
+next
+  case (tcd_lam t\<^sub>1 e t\<^sub>2)
+  have "SS False s (DLam t\<^sub>1 e) \<leadsto>\<^sub>s SS True s (DLam t\<^sub>1 e)" by simp
+  thus ?case by fastforce
+next
   case (tcd_app e\<^sub>1 t\<^sub>1 t\<^sub>2 e\<^sub>2)
-  have "SS s (DApp e\<^sub>1 e\<^sub>2) \<leadsto>\<^sub>s SS (FApp1 e\<^sub>2 # s) e\<^sub>1" by simp
-  then show ?case by fastforce
+  have "SS False s (DApp e\<^sub>1 e\<^sub>2) \<leadsto>\<^sub>s SS False (FApp1 e\<^sub>2 # s) e\<^sub>1" by simp
+  thus ?case by fastforce
 qed simp_all
 
-lemma [simp]: "s : t' \<rightarrow> t \<Longrightarrow> [] \<turnstile>\<^sub>d e : t' \<Longrightarrow> vald e \<Longrightarrow> s = [] \<or> (\<exists>\<Sigma>'. SS s e \<leadsto>\<^sub>s \<Sigma>')"
+lemma [simp]: "s : t' \<rightarrow> t \<Longrightarrow> [] \<turnstile>\<^sub>d e : t' \<Longrightarrow> vald e \<Longrightarrow> s = [] \<or> (\<exists>\<Sigma>'. SS True s e \<leadsto>\<^sub>s \<Sigma>')"
 proof (induction s t' t rule: typecheck_stack.induct)
   case (tcs_cons_app1 e\<^sub>2 t\<^sub>1 s t\<^sub>2 t)
-  hence "SS (FApp1 e\<^sub>2 # s) e \<leadsto>\<^sub>s SS (FApp2 e # s) e\<^sub>2" by simp
+  hence "SS True (FApp1 e\<^sub>2 # s) e \<leadsto>\<^sub>s SS False (FApp2 e # s) e\<^sub>2" by simp
   thus ?case by fastforce
 next
   case (tcs_cons_app2 e\<^sub>1 t\<^sub>1 t\<^sub>2 s t)
   then obtain e\<^sub>1' where "e\<^sub>1 = DLam t\<^sub>1 e\<^sub>1' \<and> insert_at 0 t\<^sub>1 [] \<turnstile>\<^sub>d e\<^sub>1' : t\<^sub>2" by blast
-  moreover with tcs_cons_app2 have "SS (FApp2 (DLam t\<^sub>1 e\<^sub>1') # s) e \<leadsto>\<^sub>s 
-    SS (FReturn # s) (substd 0 e e\<^sub>1')" by simp
+  moreover with tcs_cons_app2 have "SS True (FApp2 (DLam t\<^sub>1 e\<^sub>1') # s) e \<leadsto>\<^sub>s 
+    SS False (FReturn # s) (substd 0 e e\<^sub>1')" by simp
   ultimately show ?case by fastforce
 next 
   case (tcs_cons_ret s t')
-  hence "SS (FReturn # s) e \<leadsto>\<^sub>s SS s e" by simp
+  hence "SS True (FReturn # s) e \<leadsto>\<^sub>s SS True s e" by simp
   thus ?case by fastforce
 qed simp_all
 
-theorem progresss: "\<Sigma> :\<^sub>s t \<Longrightarrow> (\<exists>e. \<Sigma> = SS [] e \<and> vald e) \<or> (\<exists>\<Sigma>'. \<Sigma> \<leadsto>\<^sub>s \<Sigma>')"
+theorem progresss: "\<Sigma> :\<^sub>s t \<Longrightarrow> (\<exists>e. \<Sigma> = SS True [] e \<and> vald e) \<or> (\<exists>\<Sigma>'. \<Sigma> \<leadsto>\<^sub>s \<Sigma>')"
 proof (induction \<Sigma> t rule: typecheck_stack_state.induct)
-  case (tcs_state s t' t e)
-  thus ?case by (cases "vald e") simp_all
-qed
+  case (tcs_state s t' t e b)
+  thus ?case by (cases b) simp_all
+qed 
 
 theorem preservations [simp]: "\<Sigma> \<leadsto>\<^sub>s \<Sigma>' \<Longrightarrow> \<Sigma> :\<^sub>s t \<Longrightarrow> \<Sigma>' :\<^sub>s t"
 proof (induction \<Sigma> \<Sigma>' rule: evals.induct)
@@ -68,12 +78,13 @@ proof (induction \<Sigma> \<Sigma>' rule: evals.induct)
   hence "FApp1 e\<^sub>2 # s : Arrow t\<^sub>1 t\<^sub>2 \<rightarrow> t" by simp
   with X show ?case by simp
 next
-  case (evs_app2 e\<^sub>1 e\<^sub>2 s)
-  then obtain t\<^sub>1 t\<^sub>2 where X: "[] \<turnstile>\<^sub>d e\<^sub>2 : t\<^sub>1" and "s : t\<^sub>2 \<rightarrow> t" and "[] \<turnstile>\<^sub>d e\<^sub>1 : Arrow t\<^sub>1 t\<^sub>2" by blast
+  case (evs_app2 e\<^sub>2 s e\<^sub>1)
+  then obtain t\<^sub>1 t\<^sub>2 where X: "[] \<turnstile>\<^sub>d e\<^sub>2 : t\<^sub>1" and "s : t\<^sub>2 \<rightarrow> t" and "[] \<turnstile>\<^sub>d e\<^sub>1 : Arrow t\<^sub>1 t\<^sub>2" 
+   and "vald e\<^sub>1" by blast
   with evs_app2 have "FApp2 e\<^sub>1 # s : t\<^sub>1 \<rightarrow> t" by simp
   with X show ?case by simp
 next
-  case (evs_app3 e\<^sub>2 t\<^sub>1 e\<^sub>1 s)
+  case (evs_app3 t\<^sub>1 e\<^sub>1 s e\<^sub>2)
   then obtain t\<^sub>2 where "[t\<^sub>1] \<turnstile>\<^sub>d e\<^sub>1 : t\<^sub>2" and X: "s : t\<^sub>2 \<rightarrow> t" and "[] \<turnstile>\<^sub>d e\<^sub>2 : t\<^sub>1" by fastforce
   hence "[] \<turnstile>\<^sub>d substd 0 e\<^sub>2 e\<^sub>1 : t\<^sub>2" by simp
   moreover from X have "FReturn # s : t\<^sub>2 \<rightarrow> t" by simp
@@ -83,36 +94,39 @@ qed fastforce+
 lemma [simp]: "iter (\<leadsto>\<^sub>s) \<Sigma> \<Sigma>' \<Longrightarrow> \<Sigma> :\<^sub>s t \<Longrightarrow> \<Sigma>' :\<^sub>s t"
   by (induction \<Sigma> \<Sigma>' rule: iter.induct) simp_all
 
-theorem determinisms: "\<Sigma> \<leadsto>\<^sub>s \<Sigma>' \<Longrightarrow> \<Sigma> \<leadsto>\<^sub>s \<Sigma>'' \<Longrightarrow> \<Sigma>' = \<Sigma>''"
+theorem determinisms: "\<Sigma> \<leadsto>\<^sub>s \<Sigma>' \<Longrightarrow> \<Sigma> \<leadsto>\<^sub>s \<Sigma>'' \<Longrightarrow> \<Sigma> :\<^sub>s t \<Longrightarrow> \<Sigma>' = \<Sigma>''"
 proof (induction \<Sigma> \<Sigma>' rule: evals.induct)
+  case (evs_const s k)
+  thus ?case by (induction "SS False s (DConst k)" \<Sigma>'' rule: evals.induct) simp_all
+next
+  case (evs_lam s t e)
+  thus ?case by (induction "SS False s (DLam t e)" \<Sigma>'' rule: evals.induct) simp_all
+next
   case (evs_app1 s e\<^sub>1 e\<^sub>2)
-  thus ?case by (induction "SS s (DApp e\<^sub>1 e\<^sub>2)" \<Sigma>'' rule: evals.induct) simp_all
+  thus ?case by (induction "SS False s (DApp e\<^sub>1 e\<^sub>2)" \<Sigma>'' rule: evals.induct) simp_all
 next
-  case (evs_app2 e\<^sub>1 e\<^sub>2 s)
-  from evs_app2(2, 1) show ?case 
-    by (induction "SS (FApp1 e\<^sub>2 # s) e\<^sub>1" \<Sigma>'' rule: evals.induct) auto
+  case (evs_app2 e\<^sub>2 s e\<^sub>1)
+  thus ?case by (induction "SS True (FApp1 e\<^sub>2 # s) e\<^sub>1" \<Sigma>'' rule: evals.induct) simp_all
 next
-  case (evs_app3 e\<^sub>2 t e\<^sub>1 s)
-  from evs_app3(2, 1) show ?case 
-    by (induction "SS (FApp2 (DLam t e\<^sub>1) # s) e\<^sub>2" \<Sigma>'' rule: evals.induct) auto
+  case (evs_app3 t e\<^sub>1 s e\<^sub>2)
+  thus ?case by (induction "SS True (FApp2 (DLam t e\<^sub>1) # s) e\<^sub>2" \<Sigma>'' rule: evals.induct) simp_all
 next 
-  case (evs_ret e s)
-  from evs_ret(2, 1) show ?case 
-    by (induction "SS (FReturn # s) e" \<Sigma>'' rule: evals.induct) auto
+  case (evs_ret s e)
+  thus ?case by (induction "SS True (FReturn # s) e" \<Sigma>'' rule: evals.induct) simp_all
 qed
 
-lemma [simp]: "SS s e \<leadsto>\<^sub>s SS s' e' \<Longrightarrow> SS (s @ ss) e \<leadsto>\<^sub>s SS (s' @ ss) e'"
-  by (induction "SS s e" "SS s' e'" rule: evals.induct) auto
+lemma [simp]: "SS b s e \<leadsto>\<^sub>s SS b' s' e' \<Longrightarrow> SS b (s @ ss) e \<leadsto>\<^sub>s SS b' (s' @ ss) e'"
+  by (induction "SS b s e" "SS b' s' e'" rule: evals.induct) auto
 
-lemma eval_under [simp]: "iter (\<leadsto>\<^sub>s) (SS s e) (SS s' e') \<Longrightarrow> 
-  iter (\<leadsto>\<^sub>s) (SS (s @ ss) e) (SS (s' @ ss) e')"
-proof (induction "SS s e" "SS s' e'" arbitrary: s e rule: iter.induct)
+lemma eval_under [simp]: "iter (\<leadsto>\<^sub>s) (SS b s e) (SS b' s' e') \<Longrightarrow> 
+  iter (\<leadsto>\<^sub>s) (SS b (s @ ss) e) (SS b' (s' @ ss) e')"
+proof (induction "SS b s e" "SS b' s' e'" arbitrary: b s e rule: iter.induct)
   case (iter_step \<Sigma>')
   then show ?case 
   proof (induction \<Sigma>' rule: stack_state.induct)
-    case (SS s'' e'')
-    hence "SS (s @ ss) e \<leadsto>\<^sub>s SS (s'' @ ss) e''" by simp
-    moreover from SS have "iter (\<leadsto>\<^sub>s) (SS (s'' @ ss) e'') (SS (s' @ ss) e')" by simp
+    case (SS b'' s'' e'')
+    hence "SS b (s @ ss) e \<leadsto>\<^sub>s SS b'' (s'' @ ss) e''" by simp
+    moreover from SS have "iter (\<leadsto>\<^sub>s) (SS b'' (s'' @ ss) e'') (SS b' (s' @ ss) e')" by simp
     ultimately show ?case by simp
   qed
 qed simp_all
@@ -129,5 +143,24 @@ proof (induction s arbitrary: t')
     ultimately show ?case by blast
   qed force+
 qed force+
+
+lemma [simp]: "vald e \<Longrightarrow> iter (\<leadsto>\<^sub>s) (SS b s e) (SS True s e)"
+proof (induction e)
+  case (DConst x)
+  thus ?case 
+  proof (induction b)
+    case False
+    have "SS False s (DConst x) \<leadsto>\<^sub>s SS True s (DConst x)" by simp
+    thus ?case by (metis iter_step iter_refl)
+  qed simp_all
+next
+  case (DLam t e)
+  thus ?case
+  proof (induction b)
+    case False
+    have "SS False s (DLam t e) \<leadsto>\<^sub>s SS True s (DLam t e)" by simp
+    thus ?case by (metis iter_step iter_refl)
+  qed simp_all
+qed simp_all
 
 end
