04Stack/StackConversion.thy
@@ -9,7 +9,7 @@ fun unwind' :: "frame list \<Rightarrow> dexpr \<Rightarrow> dexpr" where
 | "unwind' (FReturn # s) e = unwind' s e"
 
 primrec unwind :: "stack_state \<Rightarrow> dexpr" where
-  "unwind (SS s e) = unwind' s e"
+  "unwind (SS b s e) = unwind' s e"
 
 lemma [simp]: "s : t' \<rightarrow> t \<Longrightarrow> [] \<turnstile>\<^sub>d e : t' \<Longrightarrow> [] \<turnstile>\<^sub>d unwind' s e : t"
   by (induction s t' t arbitrary: e rule: typecheck_stack.induct) simp_all
@@ -22,10 +22,10 @@ lemma [simp]: "s : t' \<rightarrow> t \<Longrightarrow> e \<leadsto>\<^sub>d e' 
 
 theorem correctd: "\<Sigma> \<leadsto>\<^sub>s \<Sigma>' \<Longrightarrow> \<Sigma> :\<^sub>s t \<Longrightarrow> iter (\<leadsto>\<^sub>d) (unwind \<Sigma>) (unwind \<Sigma>')"
 proof (induction \<Sigma> \<Sigma>' rule: evals.induct)
-  case (evs_app3 e\<^sub>2 t\<^sub>1 e\<^sub>1 s)
-  then obtain t\<^sub>2 where "s : t\<^sub>2 \<rightarrow> t" by blast
-  moreover from evs_app3 have "DApp (DLam t\<^sub>1 e\<^sub>1) e\<^sub>2 \<leadsto>\<^sub>d substd 0 e\<^sub>2 e\<^sub>1" by simp
-  ultimately have "unwind' s (DApp (DLam t\<^sub>1 e\<^sub>1) e\<^sub>2) \<leadsto>\<^sub>d unwind' s (substd 0 e\<^sub>2 e\<^sub>1)" by simp
+  case (evs_app3 t\<^sub>1 e\<^sub>1 s e\<^sub>2)
+  then obtain t\<^sub>2 where "(s : t\<^sub>2 \<rightarrow> t) \<and> vald e\<^sub>2" by blast
+  moreover hence "DApp (DLam t\<^sub>1 e\<^sub>1) e\<^sub>2 \<leadsto>\<^sub>d substd 0 e\<^sub>2 e\<^sub>1" by simp
+  ultimately have "unwind' s (DApp (DLam t\<^sub>1 e\<^sub>1) e\<^sub>2) \<leadsto>\<^sub>d unwind' s (substd 0 e\<^sub>2 e\<^sub>1)" by auto
   thus ?case by simp
 qed simp_all
 
@@ -105,7 +105,7 @@ qed simp_all
 lemma [simp]: "vald v \<Longrightarrow> v = unwind' s e \<Longrightarrow> all_returns s \<and> e = v"
   by (induction s e rule: unwind'.induct) simp_all
 
-lemma [simp]: "vald v \<Longrightarrow> v = unwind \<Sigma> \<Longrightarrow> \<exists>s. \<Sigma> = SS s v \<and> all_returns s"
+lemma [simp]: "vald v \<Longrightarrow> v = unwind \<Sigma> \<Longrightarrow> \<exists>b s. \<Sigma> = SS b s v \<and> all_returns s"
   by (induction \<Sigma>) simp_all
 
 lemma [simp]: "all_returns sr \<Longrightarrow> unwind' (s @ FApp1 e\<^sub>2 # sr) e = DApp (unwind' s e) e\<^sub>2"
@@ -114,30 +114,34 @@ lemma [simp]: "all_returns sr \<Longrightarrow> unwind' (s @ FApp1 e\<^sub>2 # s
 lemma [simp]: "all_returns sr \<Longrightarrow> unwind' (s @ FApp2 e\<^sub>1 # sr) e = DApp e\<^sub>1 (unwind' s e)"
   by (induction s e rule: unwind'.induct) auto
 
-lemma eval_returns [simp]: "all_returns sr \<Longrightarrow> vald v \<Longrightarrow> iter (\<leadsto>\<^sub>s) (SS (sr @ s) v) (SS s v)"
-proof (induction sr)
+lemma eval_returns [simp]: "all_returns sr \<Longrightarrow> vald v \<Longrightarrow> iter (\<leadsto>\<^sub>s) (SS b (sr @ s) v) (SS True s v)"
+proof (induction sr arbitrary: b)
   case (Cons a sr)
-  hence "iter (\<leadsto>\<^sub>s) (SS (sr @ s) v) (SS s v)" by simp
-  moreover from Cons have "SS (FReturn # sr @ s) v \<leadsto>\<^sub>s SS (sr @ s) v" by simp
-  ultimately have "iter (\<leadsto>\<^sub>s) (SS (FReturn # sr @ s) v) (SS s v)" by simp
+  hence "iter (\<leadsto>\<^sub>s) (SS b (FReturn # sr @ s) v) (SS True (FReturn # sr @ s) v)" by simp
+  hence "iter (\<leadsto>\<^sub>s) (SS b (FReturn # sr @ s) v) (SS True (sr @ s) v)" by simp
+  moreover from Cons have "iter (\<leadsto>\<^sub>s) (SS True (sr @ s) v) (SS True s v)" by simp
+  ultimately have "iter (\<leadsto>\<^sub>s) (SS b (FReturn # sr @ s) v) (SS True s v)" by (metis iter_append)
   with Cons show ?case by simp
 qed simp_all
 
-lemma [simp]: "unwind' s e \<leadsto>\<^sub>d e' \<Longrightarrow> s : t' \<rightarrow> t \<Longrightarrow> [] \<turnstile>\<^sub>d e : tt \<Longrightarrow> 
-  \<exists>s' e''. iter (\<leadsto>\<^sub>s) (SS s e) (SS s' e'') \<and> e' = unwind' s' e''"
-proof (induction "unwind' s e" e' arbitrary: s e t tt rule: evald.induct)
+lemma [simp]: "unwind' s e \<leadsto>\<^sub>d e' \<Longrightarrow> s : t' \<rightarrow> t \<Longrightarrow> [] \<turnstile>\<^sub>d e : tt \<Longrightarrow> (b \<Longrightarrow> vald e) \<Longrightarrow>
+  \<exists>b' s' e''. iter (\<leadsto>\<^sub>s) (SS b s e) (SS b' s' e'') \<and> e' = unwind' s' e''"
+proof (induction "unwind' s e" e' arbitrary: b s e t tt rule: evald.induct)
   case (evd_app1 e\<^sub>1 e\<^sub>1' e\<^sub>2)
   thus ?case
   proof (cases "all_returns s \<and> e = DApp e\<^sub>1 e\<^sub>2")
     case True
-    with evd_app1 True obtain t\<^sub>1 where T1: "([] \<turnstile>\<^sub>d e\<^sub>1 : Arrow t\<^sub>1 tt) \<and> ([] \<turnstile>\<^sub>d e\<^sub>2 : t\<^sub>1)" by blast
+    with evd_app1 have B: "\<not>b" by (cases b) simp_all
+    from evd_app1 True obtain t\<^sub>1 where T1: "([] \<turnstile>\<^sub>d e\<^sub>1 : Arrow t\<^sub>1 tt) \<and> ([] \<turnstile>\<^sub>d e\<^sub>2 : t\<^sub>1)" by blast
     have "[] : t' \<rightarrow> t'" by simp
-    with evd_app1 T1 obtain s' e'' where E: "iter (\<leadsto>\<^sub>s) (SS [] e\<^sub>1) (SS s' e'') \<and> 
+    with evd_app1 B T1 obtain b' s' e'' where E: "iter (\<leadsto>\<^sub>s) (SS False [] e\<^sub>1) (SS b' s' e'') \<and> 
       e\<^sub>1' = unwind' s' e''" by fastforce
-    hence "iter (\<leadsto>\<^sub>s) (SS ([] @ FApp1 e\<^sub>2 # s) e\<^sub>1) (SS (s' @ FApp1 e\<^sub>2 # s) e'')" by (metis eval_under)
-    hence "iter (\<leadsto>\<^sub>s) (SS (FApp1 e\<^sub>2 # s) e\<^sub>1) (SS (s' @ FApp1 e\<^sub>2 # s) e'')" by simp
-    hence "iter (\<leadsto>\<^sub>s) (SS s (DApp e\<^sub>1 e\<^sub>2)) (SS (s' @ FApp1 e\<^sub>2 # s) e'')" by (metis evs_app1 iter_step)
-    with True E show ?thesis by fastforce
+    hence "iter (\<leadsto>\<^sub>s) (SS False ([] @ FApp1 e\<^sub>2 # s) e\<^sub>1) (SS b' (s' @ FApp1 e\<^sub>2 # s) e'')" 
+      by (metis eval_under)
+    hence "iter (\<leadsto>\<^sub>s) (SS False (FApp1 e\<^sub>2 # s) e\<^sub>1) (SS b' (s' @ FApp1 e\<^sub>2 # s) e'')" by simp
+    hence "iter (\<leadsto>\<^sub>s) (SS False s (DApp e\<^sub>1 e\<^sub>2)) (SS b' (s' @ FApp1 e\<^sub>2 # s) e'')" 
+      by (metis evs_app1 iter_step)
+    with True B E show ?thesis by fastforce
   next
     case False
     with evd_app1 obtain s' sr where S: "all_returns sr \<and> 
@@ -147,9 +151,9 @@ proof (induction "unwind' s e" e' arbitrary: s e t tt rule: evald.induct)
     proof (cases "s = s' @ FApp1 e\<^sub>2 # sr \<and> e\<^sub>1 = unwind' s' e")
       case True
       with evd_app1 obtain t'' where "(s' : t' \<rightarrow> t'') \<and> (FApp1 e\<^sub>2 # sr : t'' \<rightarrow> t)" by fastforce
-      with evd_app1 True obtain ss' e'' where S': "iter (\<leadsto>\<^sub>s) (SS s' e) (SS ss' e'') \<and> 
+      with evd_app1 True obtain b' ss' e'' where S': "iter (\<leadsto>\<^sub>s) (SS b s' e) (SS b' ss' e'') \<and> 
         e\<^sub>1' = unwind' ss' e''" by blast
-      hence X: "iter (\<leadsto>\<^sub>s) (SS (s' @ FApp1 e\<^sub>2 # sr) e) (SS (ss' @ FApp1 e\<^sub>2 # sr) e'')" by simp
+      hence X: "iter (\<leadsto>\<^sub>s) (SS b (s' @ FApp1 e\<^sub>2 # sr) e) (SS b' (ss' @ FApp1 e\<^sub>2 # sr) e'')" by simp
       from S S' have "DApp e\<^sub>1' e\<^sub>2 = unwind' (ss' @ FApp1 e\<^sub>2 # sr) e''" by simp
       with True X show ?thesis by blast
     next
@@ -165,16 +169,19 @@ next
   thus ?case
   proof (cases "all_returns s \<and> e = DApp e\<^sub>1 e\<^sub>2")
     case True
-    with evd_app2 obtain t\<^sub>1 where T: "([] \<turnstile>\<^sub>d e\<^sub>1 : Arrow t\<^sub>1 tt) \<and> ([] \<turnstile>\<^sub>d e\<^sub>2 : t\<^sub>1)" by blast
-    from evd_app2 T obtain s' e'' where E: "iter (\<leadsto>\<^sub>s) (SS [] e\<^sub>2) (SS s' e'') \<and> 
+    with evd_app2 have B: "\<not>b" by (cases b) simp_all
+    from evd_app2 True obtain t\<^sub>1 where T: "([] \<turnstile>\<^sub>d e\<^sub>1 : Arrow t\<^sub>1 tt) \<and> ([] \<turnstile>\<^sub>d e\<^sub>2 : t\<^sub>1)" by blast
+    with evd_app2 B obtain b' s' e'' where E: "iter (\<leadsto>\<^sub>s) (SS False [] e\<^sub>2) (SS b' s' e'') \<and> 
       e\<^sub>2' = unwind' s' e''" by (metis unwind'.simps(1) tcs_nil)
-    hence "iter (\<leadsto>\<^sub>s) (SS (FApp2 e\<^sub>1 # s) e\<^sub>2) (SS (s' @ FApp2 e\<^sub>1 # s) e'')" 
+    hence "iter (\<leadsto>\<^sub>s) (SS False (FApp2 e\<^sub>1 # s) e\<^sub>2) (SS b' (s' @ FApp2 e\<^sub>1 # s) e'')" 
       by (metis eval_under append_Nil)
-    moreover have "SS s (DApp e\<^sub>1 e\<^sub>2) \<leadsto>\<^sub>s SS (FApp1 e\<^sub>2 # s) e\<^sub>1" by simp
-    moreover from evd_app2 have "SS (FApp1 e\<^sub>2 # s) e\<^sub>1 \<leadsto>\<^sub>s SS (FApp2 e\<^sub>1 # s) e\<^sub>2" by simp
-    ultimately have "iter (\<leadsto>\<^sub>s) (SS s (DApp e\<^sub>1 e\<^sub>2)) (SS (s' @ FApp2 e\<^sub>1 # s) e'')" 
-      by (metis iter_step)
-    with True E show ?thesis by fastforce
+    moreover have "SS False s (DApp e\<^sub>1 e\<^sub>2) \<leadsto>\<^sub>s SS False (FApp1 e\<^sub>2 # s) e\<^sub>1" by simp
+    moreover from evd_app2 have "iter (\<leadsto>\<^sub>s) (SS False (FApp1 e\<^sub>2 # s) e\<^sub>1) (SS True (FApp1 e\<^sub>2 # s) e\<^sub>1)" 
+      by simp
+    moreover have "SS True (FApp1 e\<^sub>2 # s) e\<^sub>1 \<leadsto>\<^sub>s SS False (FApp2 e\<^sub>1 # s) e\<^sub>2" by simp
+    ultimately have "iter (\<leadsto>\<^sub>s) (SS False s (DApp e\<^sub>1 e\<^sub>2)) (SS b' (s' @ FApp2 e\<^sub>1 # s) e'')" 
+      by (metis iter_step iter_append)
+    with True B E show ?thesis by fastforce
   next
     case False
     with evd_app2 obtain s' sr where S: "all_returns sr \<and> 
@@ -186,25 +193,28 @@ next
       with evd_app2 have S': "all_returns s' \<and> e = e\<^sub>1" by simp 
       with evd_app2 True S obtain t\<^sub>1 where T: "t' = Arrow t\<^sub>1 t \<and> [] \<turnstile>\<^sub>d e\<^sub>2 : t\<^sub>1" by blast
       have X: "e\<^sub>2 = unwind' [] e\<^sub>2" by simp
-      have "[] : t' \<rightarrow> t'" by simp
-      with evd_app2 T X obtain s'' e'' where E: "iter (\<leadsto>\<^sub>s) (SS [] e\<^sub>2) (SS s'' e'') \<and> 
+      have E: "[] : t' \<rightarrow> t'" by simp
+      have "False \<Longrightarrow> vald e\<^sub>2" by simp
+      with evd_app2 T X E obtain b'' s'' e'' where E: "iter (\<leadsto>\<^sub>s) (SS False [] e\<^sub>2) (SS b'' s'' e'') \<and> 
         e\<^sub>2' = unwind' s'' e''" by blast
-      hence "iter (\<leadsto>\<^sub>s) (SS (FApp2 e\<^sub>1 # sr) e\<^sub>2) (SS (s'' @ FApp2 e\<^sub>1 # sr) e'')" 
+      hence "iter (\<leadsto>\<^sub>s) (SS False (FApp2 e\<^sub>1 # sr) e\<^sub>2) (SS b'' (s'' @ FApp2 e\<^sub>1 # sr) e'')" 
         using eval_under by fastforce
-      moreover from evd_app2 have "SS (FApp1 e\<^sub>2 # sr) e\<^sub>1 \<leadsto>\<^sub>s SS (FApp2 e\<^sub>1 # sr) e\<^sub>2" by simp
-      moreover from evd_app2 S' have "iter (\<leadsto>\<^sub>s) (SS (s' @ FApp1 e\<^sub>2 # sr) e\<^sub>1) (SS (FApp1 e\<^sub>2 # sr) e\<^sub>1)" 
-        by simp
-      ultimately have Y: "iter (\<leadsto>\<^sub>s) (SS (s' @ FApp1 e\<^sub>2 # sr) e\<^sub>1) (SS (s'' @ FApp2 e\<^sub>1 # sr) e'')" 
-        by (metis iter_step iter_append)
+      moreover from evd_app2 have "SS True (FApp1 e\<^sub>2 # sr) e\<^sub>1 \<leadsto>\<^sub>s SS False (FApp2 e\<^sub>1 # sr) e\<^sub>2" by simp
+      moreover from evd_app2 S' have "iter (\<leadsto>\<^sub>s) (SS True (s' @ FApp1 e\<^sub>2 # sr) e\<^sub>1) 
+        (SS True (FApp1 e\<^sub>2 # sr) e\<^sub>1)" by simp
+      moreover from evd_app2 S' have "iter (\<leadsto>\<^sub>s) (SS b (s' @ FApp1 e\<^sub>2 # sr) e\<^sub>1) 
+        (SS True (s' @ FApp1 e\<^sub>2 # sr) e\<^sub>1)" by simp
+      ultimately have Y: "iter (\<leadsto>\<^sub>s) (SS b (s' @ FApp1 e\<^sub>2 # sr) e\<^sub>1) 
+        (SS b'' (s'' @ FApp2 e\<^sub>1 # sr) e'')" by (metis iter_step iter_append)
       from S E have "DApp e\<^sub>1 e\<^sub>2' = unwind' (s'' @ FApp2 e\<^sub>1 # sr) e''" by simp
-      with True S' Y show ?thesis by metis
+      with True S' Y show ?thesis by auto
     next
       case False
       with S have S': "s = s' @ FApp2 e\<^sub>1 # sr \<and> e\<^sub>2 = unwind' s' e" by simp
       with evd_app2 obtain t\<^sub>1 where "(s' : t' \<rightarrow> t\<^sub>1) \<and> (FApp2 e\<^sub>1 # sr : t\<^sub>1 \<rightarrow> t)" by fastforce
-      with evd_app2 S' obtain s'' e'' where E: "iter (\<leadsto>\<^sub>s) (SS s' e) (SS s'' e'') \<and> 
+      with evd_app2 S' obtain b'' s'' e'' where E: "iter (\<leadsto>\<^sub>s) (SS b s' e) (SS b'' s'' e'') \<and> 
         e\<^sub>2' = unwind' s'' e''" by blast
-      hence "iter (\<leadsto>\<^sub>s) (SS (s' @ FApp2 e\<^sub>1 # sr) e) (SS (s'' @ FApp2 e\<^sub>1 # sr) e'')" by simp
+      hence "iter (\<leadsto>\<^sub>s) (SS b (s' @ FApp2 e\<^sub>1 # sr) e) (SS b'' (s'' @ FApp2 e\<^sub>1 # sr) e'')" by simp
       with S S' E show ?thesis by fastforce
     qed
   qed
@@ -213,15 +223,21 @@ next
   thus ?case
   proof (cases "all_returns s \<and> e = DApp (DLam t\<^sub>1 e\<^sub>1) e\<^sub>2")
     case True
-    have "SS s (DApp (DLam t\<^sub>1 e\<^sub>1) e\<^sub>2) \<leadsto>\<^sub>s SS (FApp1 e\<^sub>2 # s) (DLam t\<^sub>1 e\<^sub>1)" by simp
-    moreover have "SS (FApp1 e\<^sub>2 # s) (DLam t\<^sub>1 e\<^sub>1) \<leadsto>\<^sub>s SS (FApp2 (DLam t\<^sub>1 e\<^sub>1) # s) e\<^sub>2" by simp
-    moreover from evd_app3 have "SS (FApp2 (DLam t\<^sub>1 e\<^sub>1) # s) e\<^sub>2 \<leadsto>\<^sub>s SS (FReturn # s) (substd 0 e\<^sub>2 e\<^sub>1)" 
+    with evd_app3 have B: "\<not>b" by (cases b) simp_all
+    have "SS False s (DApp (DLam t\<^sub>1 e\<^sub>1) e\<^sub>2) \<leadsto>\<^sub>s SS False (FApp1 e\<^sub>2 # s) (DLam t\<^sub>1 e\<^sub>1)" by simp
+    moreover have "SS False (FApp1 e\<^sub>2 # s) (DLam t\<^sub>1 e\<^sub>1) \<leadsto>\<^sub>s SS True  (FApp1 e\<^sub>2 # s) (DLam t\<^sub>1 e\<^sub>1)" 
       by simp
-    ultimately have X: "iter (\<leadsto>\<^sub>s) (SS s (DApp (DLam t\<^sub>1 e\<^sub>1) e\<^sub>2)) (SS (FReturn # s) (substd 0 e\<^sub>2 e\<^sub>1))" 
-      by (metis iter_step iter_refl)
+    moreover have "SS True (FApp1 e\<^sub>2 # s) (DLam t\<^sub>1 e\<^sub>1) \<leadsto>\<^sub>s SS False (FApp2 (DLam t\<^sub>1 e\<^sub>1) # s) e\<^sub>2" 
+      by simp
+    moreover from evd_app3 have "iter (\<leadsto>\<^sub>s) (SS False (FApp2 (DLam t\<^sub>1 e\<^sub>1) # s) e\<^sub>2) 
+      (SS True (FApp2 (DLam t\<^sub>1 e\<^sub>1) # s) e\<^sub>2)" by simp
+    moreover have "SS True (FApp2 (DLam t\<^sub>1 e\<^sub>1) # s) e\<^sub>2 \<leadsto>\<^sub>s SS False (FReturn # s) (substd 0 e\<^sub>2 e\<^sub>1)" 
+      by simp
+    ultimately have X: "iter (\<leadsto>\<^sub>s) (SS False s (DApp (DLam t\<^sub>1 e\<^sub>1) e\<^sub>2)) 
+      (SS False (FReturn # s) (substd 0 e\<^sub>2 e\<^sub>1))" by (metis iter_step iter_refl iter_append)
     from True have "substd 0 e\<^sub>2 e\<^sub>1 = unwind' (FReturn # s) (substd 0 e\<^sub>2 e\<^sub>1)"
       using unwind_returns by simp
-    with True X show ?thesis by fastforce
+    with True B X show ?thesis by fastforce
   next
     case False
     with evd_app3 obtain s' sr where S: "all_returns sr \<and> 
@@ -232,27 +248,33 @@ next
       case True
       moreover have "vald (DLam t\<^sub>1 e\<^sub>1)" by simp
       ultimately have S': "all_returns s' \<and> e = DLam t\<^sub>1 e\<^sub>1" by simp
-      have "SS (FApp1 e\<^sub>2 # sr) (DLam t\<^sub>1 e\<^sub>1) \<leadsto>\<^sub>s SS (FApp2 (DLam t\<^sub>1 e\<^sub>1) # sr) e\<^sub>2" by simp
-      moreover from evd_app3 have "SS (FApp2 (DLam t\<^sub>1 e\<^sub>1) # sr) e\<^sub>2 \<leadsto>\<^sub>s 
-        SS (FReturn # sr) (substd 0 e\<^sub>2 e\<^sub>1)" by simp
-      moreover from S' have "iter (\<leadsto>\<^sub>s) (SS (s' @ FApp1 e\<^sub>2 # sr) (DLam t\<^sub>1 e\<^sub>1)) 
-        (SS (FApp1 e\<^sub>2 # sr) (DLam t\<^sub>1 e\<^sub>1))" by simp
-      ultimately have X: "iter (\<leadsto>\<^sub>s) (SS (s' @ FApp1 e\<^sub>2 # sr) (DLam t\<^sub>1 e\<^sub>1)) 
-        (SS (FReturn # sr) (substd 0 e\<^sub>2 e\<^sub>1))" by (metis iter_step iter_refl iter_append)
+      have "SS True (FApp1 e\<^sub>2 # sr) (DLam t\<^sub>1 e\<^sub>1) \<leadsto>\<^sub>s SS False (FApp2 (DLam t\<^sub>1 e\<^sub>1) # sr) e\<^sub>2" by simp
+      moreover from evd_app3 have "iter (\<leadsto>\<^sub>s) (SS False (FApp2 (DLam t\<^sub>1 e\<^sub>1) # sr) e\<^sub>2) 
+        (SS True (FApp2 (DLam t\<^sub>1 e\<^sub>1) # sr) e\<^sub>2)" by simp
+      moreover from evd_app3 have "SS True (FApp2 (DLam t\<^sub>1 e\<^sub>1) # sr) e\<^sub>2 \<leadsto>\<^sub>s 
+        SS False (FReturn # sr) (substd 0 e\<^sub>2 e\<^sub>1)" by simp
+      moreover from S' have "iter (\<leadsto>\<^sub>s) (SS True (s' @ FApp1 e\<^sub>2 # sr) (DLam t\<^sub>1 e\<^sub>1)) 
+        (SS True (FApp1 e\<^sub>2 # sr) (DLam t\<^sub>1 e\<^sub>1))" by simp
+      moreover have "iter (\<leadsto>\<^sub>s) (SS b (s' @ FApp1 e\<^sub>2 # sr) (DLam t\<^sub>1 e\<^sub>1)) 
+        (SS True (s' @ FApp1 e\<^sub>2 # sr) (DLam t\<^sub>1 e\<^sub>1))" by simp
+      ultimately have X: "iter (\<leadsto>\<^sub>s) (SS b (s' @ FApp1 e\<^sub>2 # sr) (DLam t\<^sub>1 e\<^sub>1)) 
+        (SS False (FReturn # sr) (substd 0 e\<^sub>2 e\<^sub>1))" by (metis iter_step iter_refl iter_append)
       from S True have "substd 0 e\<^sub>2 e\<^sub>1 = unwind' (FReturn # sr) (substd 0 e\<^sub>2 e\<^sub>1)" 
         using unwind_returns by simp
       with True S' X show ?thesis by fastforce
     next
       case False
       with S evd_app3 have S': "all_returns s' \<and> e = e\<^sub>2" by simp
-      from evd_app3 have "SS (FApp2 (DLam t\<^sub>1 e\<^sub>1) # sr) e\<^sub>2 \<leadsto>\<^sub>s SS (FReturn # sr) (substd 0 e\<^sub>2 e\<^sub>1)" 
-        by simp
-      hence "iter (\<leadsto>\<^sub>s) (SS (FApp2 (DLam t\<^sub>1 e\<^sub>1) # sr) e\<^sub>2) (SS (FReturn # sr) (substd 0 e\<^sub>2 e\<^sub>1))" 
-        by (metis iter_step iter_refl)
-      moreover from evd_app3 S' have "iter (\<leadsto>\<^sub>s) (SS (s' @ FApp2 (DLam t\<^sub>1 e\<^sub>1) # sr) e\<^sub>2) 
-        (SS (FApp2 (DLam t\<^sub>1 e\<^sub>1) # sr) e\<^sub>2)" by simp
-      ultimately have X: "iter (\<leadsto>\<^sub>s) (SS (s' @ FApp2 (DLam t\<^sub>1 e\<^sub>1) # sr) e\<^sub>2) 
-        (SS (FReturn # sr) (substd 0 e\<^sub>2 e\<^sub>1))" by (metis iter_append)
+      from evd_app3 have "SS True (FApp2 (DLam t\<^sub>1 e\<^sub>1) # sr) e\<^sub>2 \<leadsto>\<^sub>s 
+        SS False (FReturn # sr) (substd 0 e\<^sub>2 e\<^sub>1)" by simp
+      hence "iter (\<leadsto>\<^sub>s) (SS True (FApp2 (DLam t\<^sub>1 e\<^sub>1) # sr) e\<^sub>2) 
+        (SS False (FReturn # sr) (substd 0 e\<^sub>2 e\<^sub>1))" by (metis iter_step iter_refl)
+      moreover from evd_app3 S' have "iter (\<leadsto>\<^sub>s) (SS True (s' @ FApp2 (DLam t\<^sub>1 e\<^sub>1) # sr) e\<^sub>2) 
+        (SS True (FApp2 (DLam t\<^sub>1 e\<^sub>1) # sr) e\<^sub>2)" by simp
+      moreover from evd_app3 have "iter (\<leadsto>\<^sub>s) (SS b (s' @ FApp2 (DLam t\<^sub>1 e\<^sub>1) # sr) e\<^sub>2) 
+        (SS True (s' @ FApp2 (DLam t\<^sub>1 e\<^sub>1) # sr) e\<^sub>2)" by simp
+      ultimately have X: "iter (\<leadsto>\<^sub>s) (SS b (s' @ FApp2 (DLam t\<^sub>1 e\<^sub>1) # sr) e\<^sub>2) 
+        (SS False (FReturn # sr) (substd 0 e\<^sub>2 e\<^sub>1))" by (metis iter_append)
       from S have "substd 0 e\<^sub>2 e\<^sub>1 = unwind' (FReturn # sr) (substd 0 e\<^sub>2 e\<^sub>1)" 
         using unwind_returns by simp
       with S False S' X show ?thesis by metis
@@ -262,8 +284,8 @@ qed
 
 theorem completed [simp]: "\<Sigma> :\<^sub>s t \<Longrightarrow> unwind \<Sigma> \<leadsto>\<^sub>d e' \<Longrightarrow> \<exists>\<Sigma>'. iter (\<leadsto>\<^sub>s) \<Sigma> \<Sigma>' \<and> e' = unwind \<Sigma>'"
 proof (induction \<Sigma> t rule: typecheck_stack_state.induct)
-  case (tcs_state s t' t e)
-  then obtain s' e'' where "iter (\<leadsto>\<^sub>s) (SS s e) (SS s' e'') \<and> e' = unwind' s' e''" by fastforce
+  case (tcs_state s t' t e b)
+  then obtain b' s' e'' where "iter (\<leadsto>\<^sub>s) (SS b s e) (SS b' s' e'') \<and> e' = unwind' s' e''" by fastforce
   thus ?case by fastforce
 qed
 
@@ -277,16 +299,17 @@ proof (induction "unwind \<Sigma>" e' arbitrary: \<Sigma> rule: iter.induct)
   then show ?case by fastforce
 qed force+
 
-lemma [simp]: "iter (\<leadsto>\<^sub>d) e v \<Longrightarrow> [] \<turnstile>\<^sub>d e : t \<Longrightarrow> vald v \<Longrightarrow> iter (\<leadsto>\<^sub>s) (SS [FReturn] e) (SS [] v)"
+lemma [simp]: "iter (\<leadsto>\<^sub>d) e v \<Longrightarrow> [] \<turnstile>\<^sub>d e : t \<Longrightarrow> vald v \<Longrightarrow> 
+  iter (\<leadsto>\<^sub>s) (SS False [FReturn] e) (SS True [] v)"
 proof -
   assume "[] \<turnstile>\<^sub>d e : t"
-  hence "SS [FReturn] e :\<^sub>s t" by (metis tcs_nil tcs_cons_ret tcs_state)
+  hence "SS False [FReturn] e :\<^sub>s t" by (metis tcs_nil tcs_cons_ret tcs_state)
   moreover assume "iter (\<leadsto>\<^sub>d) e v"
-  ultimately obtain \<Sigma>' where S: "iter (\<leadsto>\<^sub>s) (SS [FReturn] e) \<Sigma>' \<and> v = unwind \<Sigma>'" by fastforce
+  ultimately obtain \<Sigma>' where S: "iter (\<leadsto>\<^sub>s) (SS False [FReturn] e) \<Sigma>' \<and> v = unwind \<Sigma>'" by fastforce
   moreover assume V: "vald v"
-  ultimately obtain sr where "\<Sigma>' = SS (sr @ []) v \<and> all_returns sr" by fastforce
-  moreover with V have "iter (\<leadsto>\<^sub>s) \<Sigma>' (SS [] v)" by (metis eval_returns)
-  with S show "iter (\<leadsto>\<^sub>s) (SS [FReturn] e) (SS [] v)" by (metis iter_append)
+  ultimately obtain b sr where "\<Sigma>' = SS b (sr @ []) v \<and> all_returns sr" by fastforce
+  moreover with V have "iter (\<leadsto>\<^sub>s) \<Sigma>' (SS True [] v)" by (metis eval_returns)
+  with S show "iter (\<leadsto>\<^sub>s) (SS False [FReturn] e) (SS True [] v)" by (metis iter_append)
 qed
 
 end
