05Closure/ClosureConversion.thy
@@ -13,8 +13,8 @@ fun declosure_stack :: "cframe list \<Rightarrow> frame list" where
 | "declosure_stack (CReturn cs # s) = FReturn # declosure_stack s"
 
 primrec declosure_state :: "closure_state \<Rightarrow> stack_state" where
-  "declosure_state (CSE s cs e) = SS (declosure_stack s) (multisubst (map declosure cs) e)"
-| "declosure_state (CSC s c) = SS (declosure_stack s) (declosure c)"
+  "declosure_state (CSE s cs e) = SS False (declosure_stack s) (multisubst (map declosure cs) e)"
+| "declosure_state (CSC s c) = SS True (declosure_stack s) (declosure c)"
 
 lemma [simp]: "vald (declosure c)"
 proof (induction c)
@@ -90,23 +90,32 @@ proof (induction \<Sigma> \<Sigma>' rule: evalc.induct)
   ultimately have "multisubst (map declosure cs) (DVar x) = declosure c" by (metis multisubst_var)
   thus ?case by simp
 next
+  case (evc_lam s cs t e)
+  obtain e' where "multisubst (map declosure cs) (DLam t e) = DLam t e'" by fastforce
+  hence "SS False (declosure_stack s) (multisubst (map declosure cs) (DLam t e)) \<leadsto>\<^sub>s
+    SS True (declosure_stack s) (multisubst (map declosure cs) (DLam t e))" by simp
+  hence "iter (\<leadsto>\<^sub>s) (SS False (declosure_stack s) (multisubst (map declosure cs) (DLam t e)))
+    (SS True (declosure_stack s) (multisubst (map declosure cs) (DLam t e)))" 
+      by (metis iter_step iter_refl)
+  thus ?case by simp
+next
   case (evc_app s cs e\<^sub>1 e\<^sub>2)
-  have "SS (declosure_stack s) (DApp (multisubst (map declosure cs) e\<^sub>1) 
+  have "SS False (declosure_stack s) (DApp (multisubst (map declosure cs) e\<^sub>1) 
     (multisubst (map declosure cs) e\<^sub>2)) \<leadsto>\<^sub>s 
-      SS (FApp1 (multisubst (map declosure cs) e\<^sub>2) # declosure_stack s) 
+      SS False (FApp1 (multisubst (map declosure cs) e\<^sub>2) # declosure_stack s) 
         (multisubst (map declosure cs) e\<^sub>1)" by simp
-  hence "iter (\<leadsto>\<^sub>s) (SS (declosure_stack s) (DApp (multisubst (map declosure cs) e\<^sub>1) 
+  hence "iter (\<leadsto>\<^sub>s) (SS False (declosure_stack s) (DApp (multisubst (map declosure cs) e\<^sub>1) 
     (multisubst (map declosure cs) e\<^sub>2))) 
-      (SS (FApp1 (multisubst (map declosure cs) e\<^sub>2) # declosure_stack s) 
+      (SS False (FApp1 (multisubst (map declosure cs) e\<^sub>2) # declosure_stack s) 
         (multisubst (map declosure cs) e\<^sub>1))" by (metis iter_step iter_refl)
   thus ?case by simp
 next
   case (retc_app1 cs e\<^sub>2 s c\<^sub>1)
-  have "SS (FApp1 (multisubst (map declosure cs) e\<^sub>2) # declosure_stack s) (declosure c\<^sub>1) \<leadsto>\<^sub>s
-    SS (FApp2 (declosure c\<^sub>1) # declosure_stack s) (multisubst (map declosure cs) e\<^sub>2)" by simp
-  hence "iter (\<leadsto>\<^sub>s) (SS (FApp1 (multisubst (map declosure cs) e\<^sub>2) # declosure_stack s) 
+  have "SS True (FApp1 (multisubst (map declosure cs) e\<^sub>2) # declosure_stack s) (declosure c\<^sub>1) \<leadsto>\<^sub>s
+    SS False (FApp2 (declosure c\<^sub>1) # declosure_stack s) (multisubst (map declosure cs) e\<^sub>2)" by simp
+  hence "iter (\<leadsto>\<^sub>s) (SS True (FApp1 (multisubst (map declosure cs) e\<^sub>2) # declosure_stack s) 
     (declosure c\<^sub>1)) 
-      (SS (FApp2 (declosure c\<^sub>1) # declosure_stack s) (multisubst (map declosure cs) e\<^sub>2))" 
+      (SS False (FApp2 (declosure c\<^sub>1) # declosure_stack s) (multisubst (map declosure cs) e\<^sub>2))" 
         by (metis iter_step iter_refl)
   thus ?case by simp
 next
@@ -120,22 +129,22 @@ next
   with T have "multisubst (map declosure cs) (DLam t\<^sub>1 e\<^sub>1) = DLam t\<^sub>1 e' \<and> 
     multisubst (insert_at 0 (declosure c\<^sub>2) (map declosure cs)) e\<^sub>1 = substd 0 (declosure c\<^sub>2) e'" 
       by simp
-  hence "SS (FApp2 (multisubst (map declosure cs) (DLam t\<^sub>1 e\<^sub>1)) # declosure_stack s) (declosure c\<^sub>2) 
-    \<leadsto>\<^sub>s (SS (FReturn # declosure_stack s) 
+  hence "SS True (FApp2 (multisubst (map declosure cs) (DLam t\<^sub>1 e\<^sub>1)) # declosure_stack s) 
+    (declosure c\<^sub>2) \<leadsto>\<^sub>s (SS False (FReturn # declosure_stack s) 
       (multisubst (map declosure cs) (substd 0 (declosure c\<^sub>2) e\<^sub>1)))" 
     by (induction cs) simp_all
-  hence "iter (\<leadsto>\<^sub>s) (SS (FApp2 (multisubst (map declosure cs) (DLam t\<^sub>1 e\<^sub>1)) # declosure_stack s) 
+  hence "iter (\<leadsto>\<^sub>s) (SS True (FApp2 (multisubst (map declosure cs) (DLam t\<^sub>1 e\<^sub>1)) # declosure_stack s) 
     (declosure c\<^sub>2)) 
-      (SS (FReturn # declosure_stack s) 
+      (SS False (FReturn # declosure_stack s) 
         (multisubst (map declosure cs) (substd 0 (declosure c\<^sub>2) e\<^sub>1)))" 
     by (metis iter_step iter_refl)
   thus ?case by simp
 next
   case (retc_ret cs s c)
-  have "SS (FReturn # declosure_stack s) (declosure c) \<leadsto>\<^sub>s SS (declosure_stack s) (declosure c)" 
-    by simp
-  hence "iter (\<leadsto>\<^sub>s) (SS (FReturn # declosure_stack s) (declosure c)) 
-    (SS (declosure_stack s) (declosure c))" by (metis iter_step iter_refl)
+  have "SS True (FReturn # declosure_stack s) (declosure c) \<leadsto>\<^sub>s 
+    SS True (declosure_stack s) (declosure c)" by simp
+  hence "iter (\<leadsto>\<^sub>s) (SS True (FReturn # declosure_stack s) (declosure c)) 
+    (SS True (declosure_stack s) (declosure c))" by (metis iter_step iter_refl)
   thus ?case by simp
 qed simp_all
 
@@ -153,9 +162,10 @@ lemma [simp]: "FApp2 e # s = declosure_stack s\<^sub>c \<Longrightarrow>
 lemma [simp]: "FReturn # s = declosure_stack s\<^sub>c \<Longrightarrow> \<exists>cs s\<^sub>c'. s\<^sub>c = CReturn cs # s\<^sub>c'"
   by (induction s\<^sub>c rule: declosure_stack.induct) simp_all
 
-lemma [simp]: "SS s e = declosure_state \<Sigma> \<Longrightarrow> 
-  \<exists>s'. s = declosure_stack s' \<and> ((\<exists>cs e'. \<Sigma> = CSE s' cs e' \<and> e = multisubst (map declosure cs) e') \<or> 
-    (\<exists>c. \<Sigma> = CSC s' c \<and> e = declosure c))"
+lemma [dest]: "SS b s e = declosure_state \<Sigma> \<Longrightarrow> 
+  \<exists>s'. s = declosure_stack s' \<and> 
+    ((\<exists>cs e'. \<not> b \<and> \<Sigma> = CSE s' cs e' \<and> e = multisubst (map declosure cs) e') \<or> 
+      (\<exists>c. b \<and> \<Sigma> = CSC s' c \<and> e = declosure c))"
   by (induction \<Sigma>) simp_all
 
 lemma [dest]: "DApp e\<^sub>1 e\<^sub>2 = multisubst (map declosure cs) (DLam t e) \<Longrightarrow> False"
@@ -193,6 +203,88 @@ lemma [simp]: "DApp e\<^sub>1 e\<^sub>2 = multisubst (map declosure cs) e \<Long
     e\<^sub>1 = multisubst (map declosure cs) e\<^sub>1' \<and> e\<^sub>2 = multisubst (map declosure cs) e\<^sub>2'"
   by (induction e) auto
 
+lemma [dest]: "DConst k = multisubst es (declosure c) \<Longrightarrow> c = CConst k"
+proof (induction c)
+  case (CLam t cs e)
+  moreover obtain e' where "multisubst (map declosure cs) (DLam t e) = DLam t e'" by fastforce
+  moreover obtain e'' where "multisubst es (DLam t e') = DLam t e''" by fastforce
+  ultimately show ?case by simp
+qed simp_all
+
+lemma [dest]: "DConst k = multisubst (map declosure cs) (DVar x) \<Longrightarrow> lookup cs x = Some (CConst k)"
+  by (induction cs x rule: lookup.induct) auto
+
+lemma [dest]: "DConst k = multisubst (map declosure cs) e \<Longrightarrow>
+    e = DConst k \<or> (\<exists>x. e = DVar x \<and> lookup cs x = Some (CConst k))"
+proof (induction e)
+  case (DLam t e)
+  moreover then obtain e' where "multisubst (map declosure cs) (DLam t e) = DLam t e'" by force
+  ultimately show ?case by simp
+qed auto
+
+lemma [simp]: "c :\<^sub>c\<^sub>l t \<Longrightarrow> incrd x (declosure c) = declosure c"
+  and [simp]: "cs :\<^sub>c\<^sub>l\<^sub>s ts \<Longrightarrow> ts \<turnstile>\<^sub>d e : tt \<Longrightarrow> 
+    incrd x (multisubst (map declosure cs) e) = multisubst (map declosure cs) e"
+proof (induction c t and cs ts arbitrary: and e tt 
+       rule: typecheck_closure_typecheck_closure_list.inducts)
+  case (tcc_lam cs ts t\<^sub>1 e t\<^sub>2)
+  moreover hence "ts \<turnstile>\<^sub>d DLam t\<^sub>1 e : Arrow t\<^sub>1 t\<^sub>2" by simp
+  ultimately have "incrd x (multisubst (map declosure cs) (DLam t\<^sub>1 e)) = 
+    multisubst (map declosure cs) (DLam t\<^sub>1 e)" by blast
+  thus ?case by simp
+next
+  case (tcc_cons c t cs ts)
+  hence "[] \<turnstile>\<^sub>d declosure c : t" by simp
+  hence "ts \<turnstile>\<^sub>d declosure c : t" using tc_postpend by fastforce
+  moreover from tcc_cons have "insert_at 0 t ts \<turnstile>\<^sub>d e : tt" by (cases ts) simp_all
+  ultimately have "ts \<turnstile>\<^sub>d substd 0 (declosure c) e : tt" by simp
+  with tcc_cons show ?case by simp
+qed simp_all
+
+lemma [simp]: "c :\<^sub>c\<^sub>l t \<Longrightarrow> True"
+  and [simp]: "cs :\<^sub>c\<^sub>l\<^sub>s ts \<Longrightarrow> insert_at 0 t\<^sub>1 ts \<turnstile>\<^sub>d e : t\<^sub>2 \<Longrightarrow> 
+  multisubst (map declosure cs') (multisubst (map declosure cs) (DLam t\<^sub>1 e)) = 
+    multisubst (map declosure cs) (DLam t\<^sub>1 e)"
+proof (induction c t and cs ts arbitrary: and e 
+       rule: typecheck_closure_typecheck_closure_list.inducts)
+  case tcc_nil
+  thus ?case by (induction cs') simp_all
+next
+  case (tcc_cons c t cs ts)
+  hence "[] \<turnstile>\<^sub>d declosure c : t" by simp
+  hence "insert_at 0 t\<^sub>1 ts \<turnstile>\<^sub>d declosure c : t" using tc_postpend by fastforce
+  with tcc_cons show ?case by (cases ts) simp_all
+qed simp_all
+
+lemma [dest]: "c :\<^sub>c\<^sub>l tt \<Longrightarrow> DLam t e = multisubst (map declosure cs) (declosure c) \<Longrightarrow>
+  \<exists>cs' e'. c = CLam t cs' e' \<and> 
+    multisubst (map declosure cs') (DLam t e') = multisubst (map declosure cd) (declosure c)"
+proof (induction c)
+  case (CLam t\<^sub>1 cs' e')
+  then obtain t\<^sub>2 ts where T: "tt = Arrow t\<^sub>1 t\<^sub>2 \<and> (cs' :\<^sub>c\<^sub>l\<^sub>s ts) \<and> (insert_at 0 t\<^sub>1 ts \<turnstile>\<^sub>d e' : t\<^sub>2)" 
+    by fastforce
+  hence M: "multisubst (map declosure cs') (DLam t\<^sub>1 e') = 
+      multisubst (map declosure cd) (multisubst (map declosure cs') (DLam t\<^sub>1 e'))" by fastforce
+  obtain e2 where E: "multisubst (map declosure cs') (DLam t\<^sub>1 e') = DLam t\<^sub>1 e2" by fastforce
+  obtain e3 where "multisubst (map declosure cs) (DLam t\<^sub>1 e2) = DLam t\<^sub>1 e3" by fastforce
+  with CLam M E show ?case by simp
+qed simp_all
+
+lemma [dest]: "cs :\<^sub>c\<^sub>l\<^sub>s ts \<Longrightarrow> lookup ts x = Some tt \<Longrightarrow> 
+  DLam t e = multisubst (map declosure cs) (DVar x) \<Longrightarrow> 
+    \<exists>cs' e'. lookup cs x = Some (CLam t cs' e') \<and> 
+      multisubst (map declosure cs') (DLam t e') = multisubst (map declosure cs) (DVar x)"
+  by (induction cs x arbitrary: ts rule: lookup.induct) fastforce+
+
+lemma [dest]: "cs :\<^sub>c\<^sub>l\<^sub>s ts \<Longrightarrow> ts \<turnstile>\<^sub>d e : t' \<Longrightarrow> DLam t e' = multisubst (map declosure cs) e \<Longrightarrow> 
+  (\<exists>e''. e = DLam t e'') \<or> (\<exists>x cs' e''. e = DVar x \<and> lookup cs x = Some (CLam t cs' e'') \<and> 
+    multisubst (map declosure cs') (DLam t e'') = DLam t e')"
+proof (induction e)
+  case (DLam t e)
+  moreover then obtain e' where "multisubst (map declosure cs) (DLam t e) = DLam t e'" by fastforce
+  ultimately show ?case by simp
+qed auto
+
 lemma [simp]: "lookup cs x = Some c \<Longrightarrow> c :\<^sub>c\<^sub>l t \<Longrightarrow> 
     multisubst (map declosure cs) (DVar x) = declosure c"
   by (induction cs x rule: lookup.induct) simp_all
@@ -221,115 +313,93 @@ qed simp_all
 theorem completec [simp]: "declosure_state \<Sigma>\<^sub>c \<leadsto>\<^sub>s \<Sigma>\<^sub>s' \<Longrightarrow> \<Sigma>\<^sub>c :\<^sub>c t \<Longrightarrow> 
     \<exists>\<Sigma>\<^sub>c'. iter (\<leadsto>\<^sub>c) \<Sigma>\<^sub>c \<Sigma>\<^sub>c' \<and> \<Sigma>\<^sub>s' = declosure_state \<Sigma>\<^sub>c'"
 proof (induction "declosure_state \<Sigma>\<^sub>c" \<Sigma>\<^sub>s' rule: evals.induct)
-  case (evs_app1 s e\<^sub>1 e\<^sub>2)
-  then obtain s' where S: "s = declosure_stack s' \<and> 
-    ((\<exists>cs e'. \<Sigma>\<^sub>c = CSE s' cs e' \<and> DApp e\<^sub>1 e\<^sub>2 = multisubst (map declosure cs) e') \<or> 
-      (\<exists>c. \<Sigma>\<^sub>c = CSC s' c \<and> DApp e\<^sub>1 e\<^sub>2 = declosure c))" by fastforce
-  thus ?case 
-  proof (cases "\<exists>cs e'. \<Sigma>\<^sub>c = CSE s' cs e' \<and> DApp e\<^sub>1 e\<^sub>2 = multisubst (map declosure cs) e'")
-    case True
-    then obtain cs e\<^sub>1' e\<^sub>2' where E: "\<Sigma>\<^sub>c = CSE s' cs (DApp e\<^sub>1' e\<^sub>2') \<and>
-      e\<^sub>1 = multisubst (map declosure cs) e\<^sub>1' \<and> e\<^sub>2 = multisubst (map declosure cs) e\<^sub>2'" by fastforce                                                  
-    have "CSE s' cs (DApp e\<^sub>1' e\<^sub>2') \<leadsto>\<^sub>c CSE (CApp1 cs e\<^sub>2' # s') cs e\<^sub>1'" by simp
-    hence "iter (\<leadsto>\<^sub>c) (CSE s' cs (DApp e\<^sub>1' e\<^sub>2')) (CSE (CApp1 cs e\<^sub>2' # s') cs e\<^sub>1')" 
-      by (metis iter_refl iter_step)
-    with S E show ?thesis by fastforce
-  qed fastforce+
-next
-  case (evs_app2 e\<^sub>1 e\<^sub>2 s)
-  then obtain s\<^sub>c where S: "FApp1 e\<^sub>2 # s = declosure_stack s\<^sub>c \<and> 
-    ((\<exists>cs e'. \<Sigma>\<^sub>c = CSE s\<^sub>c cs e' \<and> e\<^sub>1 = multisubst (map declosure cs) e') \<or> 
-      (\<exists>c. \<Sigma>\<^sub>c = CSC s\<^sub>c c \<and> e\<^sub>1 = declosure c))" by fastforce
-  then obtain cs' e\<^sub>2' s\<^sub>c' where S': "s\<^sub>c = CApp1 cs' e\<^sub>2' # s\<^sub>c' \<and> 
-    e\<^sub>2 = multisubst (map declosure cs') e\<^sub>2' \<and> s = declosure_stack s\<^sub>c'" by fastforce
+  case (evs_const s k)
+  then obtain s' cs e' where S: "s = declosure_stack s' \<and> \<Sigma>\<^sub>c = CSE s' cs e' \<and> 
+    DConst k = multisubst (map declosure cs) e'" by fastforce
   thus ?case
-  proof (cases "\<exists>cs e'. \<Sigma>\<^sub>c = CSE s\<^sub>c cs e' \<and> e\<^sub>1 = multisubst (map declosure cs) e'")
+  proof (cases "e' = DConst k")
     case True
-    with S' obtain cs e' where E: "\<Sigma>\<^sub>c = CSE (CApp1 cs' e\<^sub>2' # s\<^sub>c') cs e' \<and>
-      e\<^sub>1 = multisubst (map declosure cs) e'" by fastforce
-    with evs_app2 obtain c where C: "
-      CSE (CApp1 cs' e\<^sub>2' # s\<^sub>c') cs e' \<leadsto>\<^sub>c CSC (CApp1 cs' e\<^sub>2' # s\<^sub>c') c \<and> 
-        multisubst (map declosure cs) e' = declosure c" by fastforce
-    moreover have "CSC (CApp1 cs' e\<^sub>2' # s\<^sub>c') c \<leadsto>\<^sub>c CSE (CApp2 c # s\<^sub>c') cs' e\<^sub>2'" by simp
-    ultimately have X: "iter (\<leadsto>\<^sub>c) (CSE (CApp1 cs' e\<^sub>2' # s\<^sub>c') cs e') (CSE (CApp2 c # s\<^sub>c') cs' e\<^sub>2')"
-      by (metis iter_refl iter_step)
-    from E C S' have "SS (FApp2 e\<^sub>1 # s) e\<^sub>2 = declosure_state (CSE (CApp2 c # s\<^sub>c') cs' e\<^sub>2')" by simp
-    with E X show ?thesis by blast
+    have "CSE s' cs (DConst k) \<leadsto>\<^sub>c CSC s' (CConst k)" by simp
+    hence "iter (\<leadsto>\<^sub>c) (CSE s' cs (DConst k)) (CSC s' (CConst k))" by (metis iter_refl iter_step)
+    with S True show ?thesis by fastforce
   next
     case False
-    with S S' obtain c where C: "\<Sigma>\<^sub>c = CSC (CApp1 cs' e\<^sub>2' # s\<^sub>c') c \<and> e\<^sub>1 = declosure c" by fastforce
-    have "CSC (CApp1 cs' e\<^sub>2' # s\<^sub>c') c \<leadsto>\<^sub>c CSE (CApp2 c # s\<^sub>c') cs' e\<^sub>2'" by simp
-    hence "iter (\<leadsto>\<^sub>c) (CSC (CApp1 cs' e\<^sub>2' # s\<^sub>c') c) (CSE (CApp2 c # s\<^sub>c') cs' e\<^sub>2')" 
-      by (metis iter_refl iter_step)
-    with C S' show ?thesis by fastforce
+    with S obtain x where E: "e' = DVar x \<and> lookup cs x = Some (CConst k)" by fastforce
+    hence "CSE s' cs (DVar x) \<leadsto>\<^sub>c CSC s' (CConst k)" by simp
+    hence X: "iter (\<leadsto>\<^sub>c) (CSE s' cs (DVar x)) (CSC s' (CConst k))" by simp
+    from S have "SS True s (DConst k) = declosure_state (CSC s' (CConst k))" by simp
+    with S E X show ?thesis by blast
   qed
 next
-  case (evs_app3 e\<^sub>2 t\<^sub>1 e\<^sub>1 s)
-  then obtain s\<^sub>c where S: "FApp2 (DLam t\<^sub>1 e\<^sub>1) # s = declosure_stack s\<^sub>c \<and> 
-    ((\<exists>cs e'. \<Sigma>\<^sub>c = CSE s\<^sub>c cs e' \<and> e\<^sub>2 = multisubst (map declosure cs) e') \<or> 
-      (\<exists>c. \<Sigma>\<^sub>c = CSC s\<^sub>c c \<and> e\<^sub>2 = declosure c))" by fastforce
+  case (evs_lam s tt e)
+  then obtain s' cs e' where S: "s = declosure_stack s' \<and> \<Sigma>\<^sub>c = CSE s' cs e' \<and> 
+    DLam tt e = multisubst (map declosure cs) e'" by fastforce
+  with evs_lam obtain t' ts where T: "(s' :\<^sub>c t' \<rightarrow> t) \<and> (cs :\<^sub>c\<^sub>l\<^sub>s ts) \<and> 
+    latest_environment s' = Some cs \<and> ts \<turnstile>\<^sub>d e' : t'" by fastforce
+  thus ?case
+  proof (cases "\<exists>e''. e' = DLam tt e''")
+    case True
+    then obtain e'' where E: "e' = DLam tt e''" by fastforce
+    have "CSE s' cs (DLam tt e'') \<leadsto>\<^sub>c CSC s' (CLam tt cs e'')" by simp
+    hence "iter (\<leadsto>\<^sub>c) (CSE s' cs (DLam tt e'')) (CSC s' (CLam tt cs e''))" 
+      by (metis iter_refl iter_step)
+    with S E show ?thesis by fastforce
+  next
+    case False
+    with S T obtain x cs' e'' where E: "e' = DVar x \<and> lookup cs x = Some (CLam tt cs' e'') \<and> 
+      multisubst (map declosure cs') (DLam tt e'') = DLam tt e" by blast
+    hence "CSE s' cs (DVar x) \<leadsto>\<^sub>c CSC s' (CLam tt cs' e'')" by simp
+    hence X: "iter (\<leadsto>\<^sub>c) (CSE s' cs (DVar x)) (CSC s' (CLam tt cs' e''))" by simp
+    from S E have "multisubst (map declosure cs) e' = multisubst (map declosure cs') (DLam tt e'')"
+      by metis
+    with S have "SS True s (DLam tt e) = declosure_state (CSC s' (CLam tt cs' e''))" by simp
+    with S E X show ?thesis by blast
+  qed
+next
+  case (evs_app1 s e\<^sub>1 e\<^sub>2)
+  then obtain s' cs e' where S: "s = declosure_stack s' \<and> \<Sigma>\<^sub>c = CSE s' cs e' \<and> 
+    DApp e\<^sub>1 e\<^sub>2 = multisubst (map declosure cs) e'" by fastforce
+  then obtain e\<^sub>1' e\<^sub>2' where E: "e' = DApp e\<^sub>1' e\<^sub>2' \<and>
+    e\<^sub>1 = multisubst (map declosure cs) e\<^sub>1' \<and> e\<^sub>2 = multisubst (map declosure cs) e\<^sub>2'" by fastforce                                                  
+  have "CSE s' cs (DApp e\<^sub>1' e\<^sub>2') \<leadsto>\<^sub>c CSE (CApp1 cs e\<^sub>2' # s') cs e\<^sub>1'" by simp
+  hence "iter (\<leadsto>\<^sub>c) (CSE s' cs (DApp e\<^sub>1' e\<^sub>2')) (CSE (CApp1 cs e\<^sub>2' # s') cs e\<^sub>1')" 
+    by (metis iter_refl iter_step)
+  with S E show ?case by fastforce
+next
+  case (evs_app2 e\<^sub>2 s e\<^sub>1)
+  then obtain s\<^sub>c c where S: "FApp1 e\<^sub>2 # s = declosure_stack s\<^sub>c \<and> \<Sigma>\<^sub>c = CSC s\<^sub>c c \<and> e\<^sub>1 = declosure c"
+    by fastforce
+  then obtain cs' e\<^sub>2' s\<^sub>c' where S': "s\<^sub>c = CApp1 cs' e\<^sub>2' # s\<^sub>c' \<and> 
+    e\<^sub>2 = multisubst (map declosure cs') e\<^sub>2' \<and> s = declosure_stack s\<^sub>c'" by fastforce
+  have "CSC (CApp1 cs' e\<^sub>2' # s\<^sub>c') c \<leadsto>\<^sub>c CSE (CApp2 c # s\<^sub>c') cs' e\<^sub>2'" by simp
+  hence "iter (\<leadsto>\<^sub>c) (CSC (CApp1 cs' e\<^sub>2' # s\<^sub>c') c) (CSE (CApp2 c # s\<^sub>c') cs' e\<^sub>2')" 
+    by (metis iter_refl iter_step)
+  with S S' show ?case by fastforce
+next
+  case (evs_app3 t\<^sub>1 e\<^sub>1 s e\<^sub>2)
+  then obtain s\<^sub>c c\<^sub>2 where S: "FApp2 (DLam t\<^sub>1 e\<^sub>1) # s = declosure_stack s\<^sub>c \<and> \<Sigma>\<^sub>c = CSC s\<^sub>c c\<^sub>2 \<and> 
+    e\<^sub>2 = declosure c\<^sub>2" by fastforce
   then obtain c s\<^sub>c' where S': "s\<^sub>c = CApp2 c # s\<^sub>c' \<and> DLam t\<^sub>1 e\<^sub>1 = declosure c \<and> 
     s = declosure_stack s\<^sub>c'" by fastforce
   then obtain cs' e\<^sub>1' where C: "c = CLam t\<^sub>1 cs' e\<^sub>1' \<and> (\<forall>e\<^sub>2. (\<forall>ee. substd 0 ee e\<^sub>2 = e\<^sub>2) \<longrightarrow> 
     substd 0 e\<^sub>2 e\<^sub>1 = multisubst (map declosure cs') (substd 0 e\<^sub>2 e\<^sub>1'))" by fastforce
-  thus ?case
-  proof (cases "(\<exists>cs e'. \<Sigma>\<^sub>c = CSE s\<^sub>c cs e' \<and> e\<^sub>2 = multisubst (map declosure cs) e')")
-    case True
-    with S' obtain cs e' where E: "\<Sigma>\<^sub>c = CSE (CApp2 c # s\<^sub>c') cs e' \<and> 
-      e\<^sub>2 = multisubst (map declosure cs) e'" by fastforce
-    with evs_app3 obtain c' where C': "CSE (CApp2 c # s\<^sub>c') cs e' \<leadsto>\<^sub>c CSC (CApp2 c # s\<^sub>c') c' \<and> 
-      multisubst (map declosure cs) e' = declosure c'" by fastforce
-    with E have E2: "e\<^sub>2 = declosure c'" by simp
-    have "CSC (CApp2 (CLam t\<^sub>1 cs' e\<^sub>1') # s\<^sub>c') c' \<leadsto>\<^sub>c CSE (CReturn (c' # cs') # s\<^sub>c') (c' # cs') e\<^sub>1'"
-      by simp
-    with C C' have X: "iter (\<leadsto>\<^sub>c) (CSE (CApp2 c # s\<^sub>c') cs e') 
-      (CSE (CReturn (c' # cs') # s\<^sub>c') (c' # cs') e\<^sub>1')" by (metis iter_step iter_refl)
-    from evs_app3 E C' have "CSC (CApp2 c # s\<^sub>c') c' :\<^sub>c t" by (metis preservationc)
-    then obtain t' where "((CApp2 c # s\<^sub>c') :\<^sub>c t' \<rightarrow> t) \<and> (c' :\<^sub>c\<^sub>l t')" by fastforce
-    with E2 have "\<forall>ee. substd 0 ee e\<^sub>2 = e\<^sub>2" by auto
-    with C S' E C' have "SS (FReturn # s) (substd 0 e\<^sub>2 e\<^sub>1) = 
-      declosure_state (CSE (CReturn (c' # cs') # s\<^sub>c') (c' # cs') e\<^sub>1')" by simp
-    with E X show ?thesis by blast
-  next
-    case False
-    with S S' C obtain c\<^sub>2 where E: "\<Sigma>\<^sub>c = CSC (CApp2 (CLam t\<^sub>1 cs' e\<^sub>1') # s\<^sub>c') c\<^sub>2 \<and> e\<^sub>2 = declosure c\<^sub>2" 
-      by fastforce
-    have X: "CSC (CApp2 (CLam t\<^sub>1 cs' e\<^sub>1') # s\<^sub>c') c\<^sub>2 \<leadsto>\<^sub>c CSE (CReturn (c\<^sub>2 # cs') # s\<^sub>c') (c\<^sub>2 # cs') e\<^sub>1'"
-      by simp
-    with evs_app3 E have "CSE (CReturn (c\<^sub>2 # cs') # s\<^sub>c') (c\<^sub>2 # cs') e\<^sub>1' :\<^sub>c t" by (metis preservationc)
-    then obtain t' ts where "(s\<^sub>c' :\<^sub>c t' \<rightarrow> t) \<and> (c\<^sub>2 # cs' :\<^sub>c\<^sub>l\<^sub>s ts) \<and> (ts \<turnstile>\<^sub>d e\<^sub>1' : t')" by fastforce
-    with E have "\<forall>ee. substd 0 ee e\<^sub>2 = e\<^sub>2" by auto
-    with S' C E have "SS (FReturn # s) (substd 0 e\<^sub>2 e\<^sub>1) = 
-      declosure_state (CSE (CReturn (c\<^sub>2 # cs') # s\<^sub>c') (c\<^sub>2 # cs') e\<^sub>1')" by simp
-    with E X show ?thesis by (metis iter_step iter_refl)
-  qed
+  have X: "CSC (CApp2 (CLam t\<^sub>1 cs' e\<^sub>1') # s\<^sub>c') c\<^sub>2 \<leadsto>\<^sub>c CSE (CReturn (c\<^sub>2 # cs') # s\<^sub>c') (c\<^sub>2 # cs') e\<^sub>1'"
+    by simp
+  with evs_app3 S S' C have "CSE (CReturn (c\<^sub>2 # cs') # s\<^sub>c') (c\<^sub>2 # cs') e\<^sub>1' :\<^sub>c t" 
+    by (metis preservationc)
+  then obtain t' ts where "(s\<^sub>c' :\<^sub>c t' \<rightarrow> t) \<and> (c\<^sub>2 # cs' :\<^sub>c\<^sub>l\<^sub>s ts) \<and> (ts \<turnstile>\<^sub>d e\<^sub>1' : t')" by fastforce
+  with S have "\<forall>ee. substd 0 ee e\<^sub>2 = e\<^sub>2" by fastforce
+  with S S' C have "SS False (FReturn # s) (substd 0 e\<^sub>2 e\<^sub>1) = 
+    declosure_state (CSE (CReturn (c\<^sub>2 # cs') # s\<^sub>c') (c\<^sub>2 # cs') e\<^sub>1')" by simp
+  with S S' C X show ?case by (metis iter_step iter_refl)
 next
-  case (evs_ret e s)
-  then obtain s\<^sub>c where S: "FReturn # s = declosure_stack s\<^sub>c \<and> 
-    ((\<exists>cs e'. \<Sigma>\<^sub>c = CSE s\<^sub>c cs e' \<and> e = multisubst (map declosure cs) e') \<or> 
-      (\<exists>c. \<Sigma>\<^sub>c = CSC s\<^sub>c c \<and> e = declosure c))" by fastforce
+  case (evs_ret s e)
+  then obtain s\<^sub>c c where S: "FReturn # s = declosure_stack s\<^sub>c \<and> \<Sigma>\<^sub>c = CSC s\<^sub>c c \<and> e = declosure c" 
+    by fastforce
   then obtain cs s\<^sub>c' where S': "s\<^sub>c = CReturn cs # s\<^sub>c'" by fastforce
-  thus ?case
-  proof (cases "(\<exists>cs' e'. \<Sigma>\<^sub>c = CSE (CReturn cs # s\<^sub>c') cs' e' \<and> 
-      e = multisubst (map declosure cs') e')")
-    case True
-    then obtain cs' e' where C: "\<Sigma>\<^sub>c = CSE (CReturn cs # s\<^sub>c') cs' e' \<and> 
-      e = multisubst (map declosure cs') e'" by fastforce
-    with evs_ret obtain c where C': "CSE (CReturn cs # s\<^sub>c') cs' e' \<leadsto>\<^sub>c CSC (CReturn cs # s\<^sub>c') c \<and> 
-      multisubst (map declosure cs') e' = declosure c" by fastforce
-    moreover have "CSC (CReturn cs # s\<^sub>c') c \<leadsto>\<^sub>c CSC s\<^sub>c' c" by simp
-    ultimately have "iter (\<leadsto>\<^sub>c) (CSE (CReturn cs # s\<^sub>c') cs' e') (CSC s\<^sub>c' c)" 
-      by (metis iter_refl iter_step)
-    with S S' C C' have "iter (\<leadsto>\<^sub>c) (CSE (CReturn cs # s\<^sub>c') cs' e') (CSC s\<^sub>c' c) \<and> 
-      SS s e = declosure_state (CSC s\<^sub>c' c)" by simp
-    with C show ?thesis by fastforce
-  next
-    case False
-    with S S' obtain c where C: "\<Sigma>\<^sub>c = CSC (CReturn cs # s\<^sub>c') c \<and> e = declosure c" by fastforce
-    have "CSC (CReturn cs # s\<^sub>c') c \<leadsto>\<^sub>c CSC s\<^sub>c' c" by simp
-    hence "iter (\<leadsto>\<^sub>c) (CSC (CReturn cs # s\<^sub>c') c) (CSC s\<^sub>c' c)" by (metis iter_refl iter_step)
-    with S S' C show ?thesis by fastforce
-  qed
+  have "CSC (CReturn cs # s\<^sub>c') c \<leadsto>\<^sub>c CSC s\<^sub>c' c" by simp
+  hence "iter (\<leadsto>\<^sub>c) (CSC (CReturn cs # s\<^sub>c') c) (CSC s\<^sub>c' c)" by (metis iter_refl iter_step)
+  with S S' show ?case by fastforce
 qed
 
 lemma [simp]: "iter (\<leadsto>\<^sub>s) (declosure_state \<Sigma>\<^sub>c) \<Sigma>\<^sub>s' \<Longrightarrow> \<Sigma>\<^sub>c :\<^sub>c t \<Longrightarrow> 
@@ -359,27 +429,16 @@ next
   thus ?case by fastforce
 qed simp_all
 
-lemma [simp]: "\<Sigma>\<^sub>c :\<^sub>c t \<Longrightarrow> iter (\<leadsto>\<^sub>s) (declosure_state \<Sigma>\<^sub>c) (SS [] v) \<Longrightarrow> 
+lemma [simp]: "\<Sigma>\<^sub>c :\<^sub>c t \<Longrightarrow> iter (\<leadsto>\<^sub>s) (declosure_state \<Sigma>\<^sub>c) (SS True [] v) \<Longrightarrow> 
   vald v \<Longrightarrow> \<exists>c. iter (\<leadsto>\<^sub>c) \<Sigma>\<^sub>c (CSC [] c) \<and> declosure c = v"
 proof -
-  assume VD: "vald v" and TC: "\<Sigma>\<^sub>c :\<^sub>c t" and "iter (\<leadsto>\<^sub>s) (declosure_state \<Sigma>\<^sub>c) (SS [] v)"
-  then obtain \<Sigma>\<^sub>c' where E: "iter (\<leadsto>\<^sub>c) \<Sigma>\<^sub>c \<Sigma>\<^sub>c' \<and> SS [] v = declosure_state \<Sigma>\<^sub>c'" by fastforce
-  then obtain s' where "[] = declosure_stack s' \<and> 
-    ((\<exists>cs e. \<Sigma>\<^sub>c' = CSE s' cs e \<and> v = multisubst (map declosure cs) e) \<or> 
-      (\<exists>c. \<Sigma>\<^sub>c' = CSC s' c \<and> v = declosure c))" by fastforce
+  assume VD: "vald v" and TC: "\<Sigma>\<^sub>c :\<^sub>c t" and "iter (\<leadsto>\<^sub>s) (declosure_state \<Sigma>\<^sub>c) (SS True [] v)"
+  then obtain \<Sigma>\<^sub>c' where E: "iter (\<leadsto>\<^sub>c) \<Sigma>\<^sub>c \<Sigma>\<^sub>c' \<and> SS True [] v = declosure_state \<Sigma>\<^sub>c'" by fastforce
+  then obtain s' c where "[] = declosure_stack s' \<and> \<Sigma>\<^sub>c' = CSC s' c \<and> v = declosure c" by fastforce
   moreover hence "s' = []" by simp
   ultimately have S: "(\<exists>cs e. \<Sigma>\<^sub>c' = CSE [] cs e \<and> v = multisubst (map declosure cs) e) \<or> 
     (\<exists>c. \<Sigma>\<^sub>c' = CSC [] c \<and> v = declosure c)" by simp
-  with E show ?thesis 
-  proof (cases "\<exists>c. \<Sigma>\<^sub>c' = CSC [] c \<and> v = declosure c")
-    case False
-    with S obtain cs e where V: "\<Sigma>\<^sub>c' = CSE [] cs e \<and> v = multisubst (map declosure cs) e" 
-      by fastforce
-    with E TC have "CSE [] cs e :\<^sub>c t" by simp
-    with V VD obtain c where "CSE [] cs e \<leadsto>\<^sub>c CSC [] c \<and> v = declosure c" by fastforce
-    with E V have "iter (\<leadsto>\<^sub>c) \<Sigma>\<^sub>c (CSC [] c) \<and> declosure c = v" by simp
-    thus ?thesis by fastforce
-  qed fastforce+
+  with E show ?thesis by fastforce
 qed
 
 end
